spec/vfmStateScript.sml
@@ -212,13 +212,6 @@ Datatype:
    |>
 End
 
-(* TODO: this probably needs to depend on block number (for hardforks) *)
-Definition wf_account_state_def:
-  wf_account_state a
-  ⇔ a.nonce < 2 ** 64                  (* https://eips.ethereum.org/EIPS/eip-2681 *)
-  ∧ LENGTH a.code <= 2 ** 14 + 2 ** 13 (* https://eips.ethereum.org/EIPS/eip-170 *)
-End
-
 Definition empty_account_state_def:
   empty_account_state =
     <| nonce := 0
@@ -228,17 +221,7 @@ Definition empty_account_state_def:
      |>
 End
 
-Theorem wf_empty_account_state[simp]:
-  wf_account_state empty_account_state
-Proof
-  rw[empty_account_state_def, wf_account_state_def]
-QED
-
 Type evm_accounts = “:address -> account_state”
-
-Definition wf_accounts_def:
-  wf_accounts a ⇔ ∀x. wf_account_state (a x)
-End
 
 Definition lookup_account_def:
   lookup_account address (accounts: evm_accounts) = accounts address
