spec/prop/vfmExecutionInvariantsScript.sml
@@ -1,0 +1,124 @@
+open HolKernel boolLib bossLib Parse
+     vfmStateTheory vfmContextTheory vfmExecutionTheory;
+
+val () = new_theory "vfmExecutionInvariants";
+
+(* TODO: this probably needs to depend on block number (for hardforks) *)
+Definition wf_account_state_def:
+  wf_account_state a
+  ⇔ a.nonce < 2 ** 64                  (* https://eips.ethereum.org/EIPS/eip-2681 *)
+  ∧ LENGTH a.code <= 2 ** 14 + 2 ** 13 (* https://eips.ethereum.org/EIPS/eip-170 *)
+End
+
+Theorem wf_empty_account_state[simp]:
+  wf_account_state empty_account_state
+Proof
+  rw[empty_account_state_def, wf_account_state_def]
+QED
+
+Definition wf_accounts_def:
+  wf_accounts a ⇔ ∀x. wf_account_state (a x)
+End
+
+Definition wf_context_def:
+  wf_context c ⇔
+    LENGTH c.stack ≤ stack_limit ∧
+    c.gasUsed ≤ c.msgParams.gasLimit
+End
+
+Definition wf_state_def:
+  wf_state s ⇔
+    s.contexts ≠ [] ∧
+    LENGTH s.contexts ≤ context_limit ∧
+    EVERY wf_context s.contexts ∧
+    wf_accounts s.rollback.accounts
+End
+
+Theorem wf_initial_context[simp]:
+  wf_context (initial_context rb callee c s rd t)
+Proof
+  rw[wf_context_def]
+QED
+
+Theorem wf_context_apply_intrinsic_cost:
+  wf_context (apply_intrinsic_cost a c) =
+  (wf_context c ∧
+   c.gasUsed ≤ c.msgParams.gasLimit - intrinsic_cost a c.msgParams)
+Proof
+  rw[apply_intrinsic_cost_def, wf_context_def]
+QED
+
+Theorem wf_initial_state:
+  wf_accounts a ∧ initial_state d st c h b a t = SOME s
+  ⇒
+  wf_state s
+Proof
+  rw[wf_accounts_def, wf_state_def, initial_state_def,
+     pre_transaction_updates_def, update_account_def,
+     initial_rollback_def, code_from_tx_def, lookup_account_def,
+     wf_context_apply_intrinsic_cost] \\ rw[]
+  \\ gs[wf_account_state_def, combinTheory.APPLY_UPDATE_THM]
+  \\ rw[wf_context_apply_intrinsic_cost]
+QED
+
+Definition preserves_wf_state_def:
+  preserves_wf_state (m: execution_state -> α execution_result) =
+  ∀s. wf_state s ⇒ wf_state (SND (m s))
+End
+
+Theorem preserves_wf_state_handle[simp]:
+  preserves_wf_state f ∧
+  (∀e. preserves_wf_state (h e))
+  ⇒
+  preserves_wf_state (handle f h)
+Proof
+  rw[preserves_wf_state_def, handle_def]
+  \\ CASE_TAC \\ gs[]
+  \\ CASE_TAC \\ gs[]
+  \\ last_x_assum drule \\ rw[]
+QED
+
+Theorem preserves_wf_state_bind_gen:
+  preserves_wf_state g ∧
+  (∀s a s'. g s = (INL a, s') ⇒ p a) ∧
+  (∀x. p x ⇒ preserves_wf_state (f x))
+  ⇒
+  preserves_wf_state (bind g f)
+Proof
+  rw[preserves_wf_state_def, bind_def]
+  \\ CASE_TAC
+  \\ last_x_assum drule \\ rw[]
+  \\ CASE_TAC \\ rw[]
+  \\ last_x_assum drule \\ rw[]
+QED
+
+Theorem preserves_wf_state_bind:
+  preserves_wf_state g ∧
+  (∀x. preserves_wf_state (f x))
+  ⇒
+  preserves_wf_state (bind g f)
+Proof
+  strip_tac
+  \\ irule preserves_wf_state_bind_gen \\ rw[]
+  \\ qexists_tac`K T` \\ rw[]
+QED
+
+Theorem preserves_wf_state_ignore_bind:
+  preserves_wf_state g ∧ preserves_wf_state f
+  ⇒
+  preserves_wf_state (ignore_bind g f)
+Proof
+  rw[ignore_bind_def]
+  \\ irule preserves_wf_state_bind
+  \\ rw[]
+QED
+
+Theorem wf_state_step[simp]:
+  preserves_wf_state step
+Proof
+  rw[step_def]
+  \\ irule preserves_wf_state_handle
+  \\ cheat
+QED
+
+val () = export_theory();
